src/absyn/visit.fs
@@ -306,11 +306,11 @@ and reduce_exp
 
         | Exp_match(e1, pl) -> 
           let rec pat_binders b p = match p with 
-            | Pat_wild
-            | Pat_twild
+            | Pat_wild _
+            | Pat_twild _
             | Pat_constant _ -> b
             | Pat_meta(Meta_pat_pos(p, _))
-            | Pat_meta(Meta_pat_exp(p, _)) -> pat_binders b p
+            | Pat_meta(Meta_pat_exp(p, _, _)) -> pat_binders b p
             | Pat_var x -> push_vbinder b (Some x)
             | Pat_tvar t -> push_tbinder b (Some t)
             | Pat_cons(c, pats) -> List.fold_left pat_binders b pats
